CN_Lib/CN_Lib_Iris.lean
@@ -6,11 +6,9 @@ import Iris.Std.GenSetsInstances
 import Iris.ProofMode
 import Std.Data.ExtTreeMap
 import CN_Lib.CN_Lib
-import Lean.Elab
-import Lean
+import CN_Lib.CN_Lib_Tactics
 
-open Lean Elab Tactic Qq
-open Iris ProgramLogic Language.Notation Std FromMathlib BI
+open Iris ProgramLogic Language.Notation Std FromMathlib BI CN_Lib
 
 namespace CN_Lib
 
@@ -37,18 +35,18 @@ variable [MyHeap hlc GF]
 
 
 -- 2, CN-style ownership predicates.
--- Every ownership predicate reduces to ownership of unsigned
--- bytes and a proof that the value is within bounds for that type.
+--  Every ownership predicate reduces to ownership of unsigned
+--  bytes and a proof that the value is within bounds for that type.
 
--- Ownership of unsigned C integer types
+-- Unsigned C integer types
 def Owned_UChar (l : Ptr) (v : Int) : IProp GF := iprop%
     (l ↦ some v) -- Pointsto predicate
   ∗ ⌜l ≠ 0⌝ -- Pointer is non-null
   ∗ ⌜ min_UChar ≤ v ∧ v ≤ max_UChar ⌝ -- Value is within bounds
 def Owned_UShort (l : Ptr) (v : Int) : IProp GF :=
   let bytes := UShort_bytes v
-    iprop% Owned_UChar l (bytes 0)
-  ∗ Owned_UChar (l + 1) (bytes 1)
+    iprop%
+    (Owned_UChar l (bytes 0) ∗ Owned_UChar (l + 1) (bytes 1))
   ∗ ⌜ min_UShort ≤ v ∧ v ≤ max_UShort ⌝
 def Owned_UInt (l : Ptr) (v : Int) : IProp GF :=
   let bytes := UInt_bytes v
@@ -61,7 +59,7 @@ def Owned_ULong (l : Ptr) (v : Int) : IProp GF :=
     ([∗list] i ↦ b ∈ List.ofFn bytes, Owned_UChar (l + i) b)
   ∗ ⌜ min_ULong ≤ v ∧ v ≤ max_ULong ⌝
 
--- Ownership of signed C integer types
+-- Signed C integer types
 def Owned_Char (l : Ptr) (v : Int) : IProp GF :=
   let byte := wrapI min_UChar max_UChar v
   iprop%
@@ -70,8 +68,7 @@ def Owned_Char (l : Ptr) (v : Int) : IProp GF :=
 def Owned_Short (l : Ptr) (v : Int) : IProp GF :=
   let bytes := UShort_bytes (wrapI min_UShort max_UShort v)
   iprop%
-    Owned_UChar l (bytes 0)
-  ∗ Owned_UChar (l + 1) (bytes 1)
+    (Owned_UChar l (bytes 0) ∗ Owned_UChar (l + 1) (bytes 1))
   ∗ ⌜ min_Short ≤ v ∧ v ≤ max_Short ⌝
 def Owned_Int (l : Ptr) (v : Int) : IProp GF :=
   let bytes := UInt_bytes (wrapI min_UInt max_UInt v)
@@ -84,9 +81,7 @@ def Owned_Long (l : Ptr) (v : Int) : IProp GF :=
     ([∗list] i ↦ b ∈ List.ofFn bytes, Owned_UChar (l + i) b)
   ∗ ⌜ min_Long ≤ v ∧ v ≤ max_Long ⌝
 
-
 -- 3, Array ownership
-
 def Block (l : Ptr) : IProp GF := iprop% (l ↦ none) ∧ ⌜l ≠ 0⌝
 
 def arrayshift (l : Ptr) (pos : Int) (size : Int) : Ptr := l + pos * size
@@ -96,26 +91,60 @@ def padding (l : Ptr) (n : Nat) : IProp GF :=
   | 0 => l ↦ none
   | Nat.succ n' => iprop% (Block l ∗ padding (l + 1) n')
 
-
 -- 4, Pointer non-null theorems
-theorem ptr_nonnull {l : Ptr} {v : Int} :
+theorem Owned_UChar_nonnull {l : Ptr} {v : Int} :
   ⊢@{IProp GF} Owned_UChar l v → ⌜l ≠ 0⌝ :=
 by
   unfold Owned_UChar
   iintro ⟨_ , ⟨HOwn, _⟩⟩; iframe
 
--- Owned integer pointers can't be null
-theorem ptr_int_nonnull {l : Ptr} {v : Int} :
+theorem Owned_Char_nonnull {l : Ptr} {v : Int} :
+  ⊢@{IProp GF} Owned_Char l v → ⌜l ≠ 0⌝ :=
+by
+  unfold Owned_Char Owned_UChar
+  iintro ⟨⟨_ , ⟨H , _⟩⟩ , _⟩; iframe
+
+theorem Owned_UShort_nonnull {l : Ptr} {v : Int} :
+  ⊢@{IProp GF} Owned_UShort l v → ⌜l ≠ 0⌝ :=
+by
+  unfold Owned_UShort Owned_UChar
+  iintro ⟨⟨⟨_ , ⟨H , _⟩⟩ , _⟩ , _⟩; iframe
+
+theorem Owned_Short_nonnull {l : Ptr} {v : Int} :
+  ⊢@{IProp GF} Owned_Short l v → ⌜l ≠ 0⌝ :=
+by
+  unfold Owned_Short Owned_UChar
+  iintro ⟨⟨⟨_ , ⟨H , _⟩⟩ , _⟩ , _⟩; iframe
+
+theorem Owned_UInt_nonnull {l : Ptr} {v : Int} :
+  ⊢@{IProp GF} Owned_UInt l v → ⌜l ≠ 0⌝ :=
+by
+  unfold Owned_UInt Owned_UChar
+  iintro ⟨H , _⟩; simp
+  icases H with ⟨⟨_ , ⟨H , _⟩⟩ , _⟩; iframe
+
+theorem Owned_Int_nonnull {l : Ptr} {v : Int} :
   ⊢@{IProp GF} Owned_Int l v → ⌜l ≠ 0⌝ :=
 by
   unfold Owned_Int Owned_UChar
-  iintro ⟨H , _⟩
-  simp
+  iintro ⟨H , _⟩; simp
   icases H with ⟨⟨_ , ⟨H , _⟩⟩ , _⟩; iframe
 
--- TODO: fill these in
+theorem Owned_ULong_nonnull {l : Ptr} {v : Int} :
+  ⊢@{IProp GF} Owned_ULong l v → ⌜l ≠ 0⌝ :=
+by
+  unfold Owned_ULong Owned_UChar
+  iintro ⟨H , _⟩; simp
+  icases H with ⟨⟨_ , ⟨H , _⟩⟩ , _⟩; iframe
 
--- 5, Equality theorems for ownership predicates
+theorem Owned_Long_nonnull {l : Ptr} {v : Int} :
+  ⊢@{IProp GF} Owned_Long l v → ⌜l ≠ 0⌝ :=
+by
+  unfold Owned_Long Owned_UChar
+  iintro ⟨H , _⟩; simp
+  icases H with ⟨⟨_ , ⟨H , _⟩⟩ , _⟩; iframe
+
+-- 5, Value equality theorems for ownership predicates
 
 theorem Owned_UChar_eq {l : Ptr} {v v' : Int} :
   ⊢@{IProp GF} Owned_UChar l v -∗ Owned_UChar l v' -∗ ⌜v = v'⌝ :=
@@ -131,40 +160,21 @@ by
   unfold Owned_Char min_Char max_Char
   iintro ⟨H1 , %H2⟩ ⟨H3 , %H4⟩
   ihave %HEq := Owned_UChar_eq $$ H1 H3
-  ipureintro
-  apply wrapI_Char_cong H2 H4 HEq
+  ipureintro; apply wrapI_Char_cong H2 H4 HEq
 
 theorem Owned_UShort_eq {l : Ptr} {v v' : Int} :
   ⊢@{IProp GF} Owned_UShort l v -∗ Owned_UShort l v' -∗ ⌜v = v'⌝ :=
 by
-  unfold Owned_UShort min_UShort max_UShort
-  iintro ⟨H1 , ⟨H2 , ⟨%H⟩⟩⟩ ⟨H5 , ⟨H6 , ⟨%H'⟩⟩⟩
-  ihave %HEq := Owned_UChar_eq $$ H1 H5
-  ihave %HEq' := Owned_UChar_eq $$ H2 H6
-  ipureintro
-  have Hbytes : UShort_bytes v = UShort_bytes v' := by
-    funext i
-    repeat refine Fin.lastCases ?_ ?_ i; lia; intro i
-    apply Fin.elim0; assumption
-  have H := UShort_eq H H' Hbytes
-  assumption
+  unfold Owned_UShort
+  iintro ⟨HOwn, %H⟩ ⟨HOwn', %H'⟩
+  solve_owned_eq Owned_UChar_eq (HOwn, HOwn') v v' H H'
 
 theorem Owned_Short_eq {l : Ptr} {v v' : Int} :
   ⊢@{IProp GF} Owned_Short l v -∗ Owned_Short l v' -∗ ⌜v = v'⌝ :=
 by
   unfold Owned_Short
-  iintro ⟨H1 , ⟨H2 , %H⟩⟩ ⟨H3 , ⟨H4 , %H'⟩⟩
-  ihave %HEq := Owned_UChar_eq $$ H1 H3
-  ihave %HEq' := Owned_UChar_eq $$ H2 H4
-  ipureintro
-  have Hbytes : UShort_bytes (wrapI min_UShort max_UShort v) = UShort_bytes (wrapI min_UShort max_UShort v') := by
-    funext i
-    repeat refine Fin.lastCases ?_ ?_ i; lia; intro i
-    apply Fin.elim0; assumption
-  have Hv := wrapI_within_bounds (x := v) (min := min_UShort) (max := max_UShort) (by lia)
-  have Hv' := wrapI_within_bounds (x := v') (min := min_UShort) (max := max_UShort) (by lia)
-  have H1 := UShort_eq Hv Hv' Hbytes
-  apply wrapI_Short_cong H H' H1
+  iintro ⟨HOwn, %H⟩ ⟨HOwn', %H'⟩
+  solve_owned_eq Owned_UChar_eq (HOwn, HOwn') v v' H H'
 
 theorem Owned_UInt_eq {l : Ptr} {v v' : Int} :
   ⊢@{IProp GF} Owned_UInt l v -∗ Owned_UInt l v' -∗ ⌜v = v'⌝ :=
@@ -172,19 +182,7 @@ by
   unfold Owned_UInt
   iintro ⟨HOwn, %H⟩ ⟨HOwn', %H'⟩
   simp [-UInt_bytes]
-  icases HOwn with ⟨H1 , ⟨H2 , ⟨H3 , ⟨H4 , _⟩⟩⟩⟩
-  icases HOwn' with ⟨H1' , ⟨H2' , ⟨H3' , ⟨H4' , _⟩⟩⟩⟩
-  ihave %H1 := Owned_UChar_eq $$ H1 H1'
-  ihave %H2 := Owned_UChar_eq $$ H2 H2'
-  ihave %H3 := Owned_UChar_eq $$ H3 H3'
-  ihave %H4 := Owned_UChar_eq $$ H4 H4'
-  ipureintro
-  have Hbytes : UInt_bytes v = UInt_bytes v' := by
-    funext i
-    repeat refine Fin.lastCases ?_ ?_ i; lia; intro i
-    apply Fin.elim0; assumption
-  have H1 := UInt_eq H H' Hbytes
-  assumption
+  solve_owned_eq Owned_UChar_eq (HOwn, HOwn') v v' H H'
 
 theorem Owned_Int_eq {l : Ptr} {v v' : Int} :
   ⊢@{IProp GF} Owned_Int l v -∗ Owned_Int l v' -∗ ⌜v = v'⌝ :=
@@ -192,21 +190,7 @@ by
   unfold Owned_Int
   iintro ⟨HOwn, %H⟩ ⟨HOwn', %H'⟩
   simp [-UInt_bytes]
-  icases HOwn with ⟨H1 , ⟨H2 , ⟨H3 , ⟨H4 , _⟩⟩⟩⟩
-  icases HOwn' with ⟨H1' , ⟨H2' , ⟨H3' , ⟨H4' , _⟩⟩⟩⟩
-  ihave %H1 := Owned_UChar_eq $$ H1 H1'
-  ihave %H2 := Owned_UChar_eq $$ H2 H2'
-  ihave %H3 := Owned_UChar_eq $$ H3 H3'
-  ihave %H4 := Owned_UChar_eq $$ H4 H4'
-  ipureintro
-  have Hbytes : UInt_bytes (wrapI min_UInt max_UInt v) = UInt_bytes (wrapI min_UInt max_UInt v') := by
-    funext i
-    repeat refine Fin.lastCases ?_ ?_ i; lia; intro i
-    apply Fin.elim0; assumption
-  have Hv := wrapI_within_bounds (x := v) (min := min_UInt) (max := max_UInt) (by lia)
-  have Hv' := wrapI_within_bounds (x := v') (min := min_UInt) (max := max_UInt) (by lia)
-  have H1 := UInt_eq Hv Hv' Hbytes
-  apply wrapI_Int_cong H H' H1
+  solve_owned_eq Owned_UChar_eq (HOwn, HOwn') v v' H H'
 
 theorem Owned_ULong_eq {l : Ptr} {v v' : Int} :
   ⊢@{IProp GF} Owned_ULong l v -∗ Owned_ULong l v' -∗ ⌜v = v'⌝ :=
@@ -214,22 +198,58 @@ by
   unfold Owned_ULong
   iintro ⟨HOwn, %H⟩ ⟨HOwn', %H'⟩
   simp [-ULong_bytes]
-  icases HOwn with ⟨H1 , ⟨H2 , ⟨H3 , ⟨H4 , HOwn⟩⟩⟩⟩
-  icases HOwn with ⟨H5 , ⟨H6 , ⟨H7 , ⟨H8 , _⟩⟩⟩⟩
-  icases HOwn' with ⟨H1' , ⟨H2' , ⟨H3' , ⟨H4' , HOwn'⟩⟩⟩⟩
-  icases HOwn' with ⟨H5' , ⟨H6' , ⟨H7' , ⟨H8' , _⟩⟩⟩⟩
-  ihave %H1 := Owned_UChar_eq $$ H1 H1'
-  ihave %H2 := Owned_UChar_eq $$ H2 H2'
-  ihave %H3 := Owned_UChar_eq $$ H3 H3'
-  ihave %H4 := Owned_UChar_eq $$ H4 H4'
-  ihave %H5 := Owned_UChar_eq $$ H5 H5'
-  ihave %H6 := Owned_UChar_eq $$ H6 H6'
-  ihave %H7 := Owned_UChar_eq $$ H7 H7'
-  ihave %H8 := Owned_UChar_eq $$ H8 H8'
-  ipureintro
-  have Hbytes : ULong_bytes v = ULong_bytes v' := by
-    funext i
-    repeat refine Fin.lastCases ?_ ?_ i; lia; intro i
-    apply Fin.elim0; assumption
-  have H1 := ULong_eq H H' Hbytes
-  assumption
+  solve_owned_eq Owned_UChar_eq (HOwn, HOwn') v v' H H'
+
+theorem Owned_Long_eq {l : Ptr} {v v' : Int} :
+  ⊢@{IProp GF} Owned_Long l v -∗ Owned_Long l v' -∗ ⌜v = v'⌝ :=
+by
+  unfold Owned_Long
+  iintro ⟨HOwn, %H⟩ ⟨HOwn', %H'⟩
+  simp [-ULong_bytes]
+  solve_owned_eq Owned_UChar_eq (HOwn, HOwn') v v' H H'
+
+-- 6, Pointer inequality theorems for ownership predicates
+
+theorem Owned_UChar_neq {l l' : Ptr} {v v' : Int} :
+  ⊢@{IProp GF} Owned_UChar l v -∗ Owned_UChar l' v' -∗ ⌜l ≠ l'⌝ :=
+by
+  unfold Owned_UChar
+  iintro ⟨H1 , _⟩ ⟨H2 , _⟩
+  iapply pointsTo_ne $$ H1 H2
+
+theorem Owned_Char_neq {l l' : Ptr} {v v' : Int} :
+  ⊢@{IProp GF} Owned_Char l v -∗ Owned_Char l' v' -∗ ⌜l ≠ l'⌝ :=
+by
+  unfold Owned_Char
+  iintro ⟨H1 , _⟩ ⟨H2 , _⟩
+  iapply Owned_UChar_neq $$ H1 H2
+
+theorem Owned_UShort_neq {l l' : Ptr} {v v' : Int} :
+  ⊢@{IProp GF} Owned_UShort l v -∗ Owned_UShort l' v' -∗ ⌜l ≠ l'⌝ :=
+by
+  solve_own_neq Owned_UShort Owned_UChar_neq
+
+theorem Owned_Short_neq {l l' : Ptr} {v v' : Int} :
+  ⊢@{IProp GF} Owned_Short l v -∗ Owned_Short l' v' -∗ ⌜l ≠ l'⌝ :=
+by
+  solve_own_neq Owned_Short Owned_UChar_neq
+
+theorem Owned_UInt_neq {l l' : Ptr} {v v' : Int} :
+  ⊢@{IProp GF} Owned_UInt l v -∗ Owned_UInt l' v' -∗ ⌜l ≠ l'⌝ :=
+by
+  solve_own_neq Owned_UInt Owned_UChar_neq
+
+theorem Owned_Int_neq {l l' : Ptr} {v v' : Int} :
+  ⊢@{IProp GF} Owned_Int l v -∗ Owned_Int l' v' -∗ ⌜l ≠ l'⌝ :=
+by
+  solve_own_neq Owned_Int Owned_UChar_neq
+
+theorem Owned_ULong_neq {l l' : Ptr} {v v' : Int} :
+  ⊢@{IProp GF} Owned_ULong l v -∗ Owned_ULong l' v' -∗ ⌜l ≠ l'⌝ :=
+by
+  solve_own_neq Owned_ULong Owned_UChar_neq
+
+theorem Owned_Long_neq {l l' : Ptr} {v v' : Int} :
+  ⊢@{IProp GF} Owned_Long l v -∗ Owned_Long l' v' -∗ ⌜l ≠ l'⌝ :=
+by
+  solve_own_neq Owned_Long Owned_UChar_neq
