CN_Lib/CN_Lib_Tactics.lean
@@ -1,0 +1,112 @@
+import Iris.Proofmode.Tactics
+import Iris.BI.Lib.Fixpoint
+import Qq
+import Batteries.Tactic.SeqFocus
+import Lean.Elab
+import Lean
+import CN_Lib.CN_Lib
+
+open Lean Elab Tactic Qq
+
+-- This file contains some useful tactics for proofs involving CN ownership predicates over integer types.
+
+namespace CN_Lib
+
+declare_syntax_cat ident_tuple
+scoped syntax "(" ident "," ident ")":ident_tuple
+
+declare_syntax_cat pmTerm_tuple
+scoped syntax "(" pmTerm "," pmTerm ")":pmTerm_tuple
+
+scoped syntax "own_eq" ident ident_tuple* : tactic
+macro_rules
+  | `(tactic| own_eq $_) => `(tactic|skip) --no args, tactic does nothing
+  | `(tactic| own_eq $f ($hd,$hd') $[$tl]*) =>
+    `(tactic|
+        ihave %$hd := $f:ident $$ $hd:ident $hd':ident <;>
+        own_eq $f $[$tl]*)
+
+-- Tactic that destructs owned predicates into their component Owned_UChar predicates
+scoped syntax "destruct_owned" pmTerm_tuple ident : tactic
+macro_rules
+  | `(tactic| destruct_owned ($HOwn, $HOwn') $f) =>
+      `(tactic| first
+        | icases $HOwn with ⟨H1, ⟨H2, ⟨H3, ⟨H4, HOwn⟩⟩⟩⟩ <;>
+          icases HOwn with ⟨H5, ⟨H6, ⟨H7, ⟨H8, _⟩⟩⟩⟩ <;>
+          icases $HOwn' with ⟨H1', ⟨H2', ⟨H3', ⟨H4', HOwn'⟩⟩⟩⟩ <;>
+          icases HOwn' with ⟨H5', ⟨H6', ⟨H7', ⟨H8', _⟩⟩⟩⟩ <;>
+          own_eq $f (H1, H1') (H2, H2') (H3, H3') (H4, H4')
+            (H5, H5') (H6, H6') (H7, H7') (H8, H8')
+        | icases $HOwn with ⟨H1, ⟨H2, ⟨H3, ⟨H4, _⟩⟩⟩⟩ <;>
+          icases $HOwn' with ⟨H1', ⟨H2', ⟨H3', ⟨H4', _⟩⟩⟩⟩ <;>
+          own_eq $f (H1, H1') (H2, H2') (H3, H3') (H4, H4')
+        | icases $HOwn with ⟨H1, H2⟩ <;>
+          icases $HOwn' with ⟨H1', H2'⟩ <;>
+          own_eq $f (H1, H1') (H2, H2')
+          )
+
+-- Macro that proves `f v = f v'` from `f : Fin n → Int` and seperate hypotheses stating
+--  `f v i = f v' i` for each `i` in `Fin n`.
+scoped syntax "solve_fin_from_cases" : tactic
+macro_rules
+  | `(tactic| solve_fin_from_cases) =>
+    `(tactic| funext i <;>
+      (repeat refine Fin.lastCases ?_ ?_ i ; lia ; intro i) <;>
+      apply Fin.elim0 <;> assumption)
+
+-- Tactic that solves goals of the form ⌜v = v'⌝ given a pair of owned signed predicates
+elab "solve_owned_eq_signed" HOwn:pmTerm_tuple f:ident
+  f_bytes:ident min:ident max:ident
+  v:ident v':ident H:ident H':ident : tactic => do
+  evalTactic <| ← `(tactic|
+    destruct_owned $HOwn $f <;> ipureintro <;>
+    (have Hbytes : $f_bytes (wrapI $min $max $v) = $f_bytes (wrapI $min $max $v') := by
+      solve_fin_from_cases) <;>
+    have Hv := wrapI_within_bounds (x := $v) (min := $min) (max := $max) (by lia) <;>
+    have Hv' := wrapI_within_bounds (x := $v') (min := $min) (max := $max) (by lia) <;>
+    (first
+      | have HEq := CN_Lib.UShort_eq Hv Hv' Hbytes <;> apply wrapI_Short_cong $H $H' HEq
+      | have HEq := CN_Lib.UInt_eq Hv Hv' Hbytes <;> apply wrapI_Int_cong $H $H' HEq
+      | have HEq := CN_Lib.ULong_eq Hv Hv' Hbytes <;> apply wrapI_Long_cong $H $H' HEq)
+    )
+
+-- Tactic that solves goals of the form ⌜v = v'⌝ given a pair of owned unsigned predicates
+elab "solve_owned_eq_unsigned" HOwn:pmTerm_tuple f:ident
+  f_bytes:ident
+  v:ident v':ident H:ident H':ident : tactic => do
+  evalTactic <| ← `(tactic|
+    destruct_owned $HOwn $f <;> ipureintro <;>
+    (have Hbytes : $f_bytes $v = $f_bytes $v' := by
+      funext i
+      repeat refine Fin.lastCases ?_ ?_ i; lia; intro i
+      apply Fin.elim0; assumption) <;>
+    (first
+      | have HEq := CN_Lib.ULong_eq $H $H' Hbytes <;> assumption
+      | have HEq := CN_Lib.UInt_eq $H $H' Hbytes <;> assumption
+      | have HEq := CN_Lib.UShort_eq $H $H' Hbytes <;> assumption
+      )
+    )
+
+-- Tactic that tries to apply the above two tactics for each supported C integer type
+elab "solve_owned_eq" f:ident HOwn:pmTerm_tuple
+  v:ident v':ident
+  H:ident H':ident : tactic => do
+  evalTactic <| ← `(tactic|
+    (first
+      | solve_owned_eq_unsigned $HOwn $f ULong_bytes $v $v' $H $H'
+      | solve_owned_eq_unsigned $HOwn $f UInt_bytes $v $v' $H $H'
+      | solve_owned_eq_unsigned $HOwn $f UShort_bytes $v $v' $H $H'
+      | solve_owned_eq_signed $HOwn $f UInt_bytes min_UInt max_UInt $v $v' $H $H'
+      | solve_owned_eq_signed $HOwn $f UShort_bytes min_UShort max_UShort $v $v' $H $H'
+      | solve_owned_eq_signed $HOwn $f ULong_bytes min_ULong max_ULong $v $v' $H $H'
+      )
+    )
+
+-- Tactic that solves inequalities of the form ⌜l ≠ l'⌝ given a pair of owned predicates
+scoped syntax "solve_own_neq" ident ident: tactic
+macro_rules
+  | `(tactic| solve_own_neq $f $g) =>
+      `(tactic| unfold $f <;>
+          iintro ⟨H1 , _⟩ ⟨H2 , _⟩; simp <;>
+          icases H1 with ⟨H1 , _⟩; icases H2 with ⟨H2 , _⟩ <;>
+          iapply $g:ident $$ H1 H2)
